examples/layeredeffects/GT.fst
@@ -53,7 +53,7 @@ let t1_d () : Dv (list int) = downgrade_val (r_map #D (fun x -> raise_val (fun (
 
 let subcomp (a:Type) (i:idx) (f : m a i) : m a i = f
 
-let if_then_else (a:Type) (i:idx) (f : m a i) (g : m a i) (p : Type0) : Type = m a i
+let if_then_else (a:Type) (i:idx) (f : m a i) (g : m a i) (b : bool) : Type = m a i
 
 // GM: Would be nice to not have to use all explicit args everywhere,
 //     and to get better errors especially when args are out of order,
@@ -73,7 +73,7 @@ layered_effect {
 }
 
 let lift_pure_gtd (a:Type) (wp : pure_wp a) (i : idx)
-                  (f : unit -> PURE a wp)
+                  (f : eqtype_as_type unit -> PURE a wp)
                  : Pure (m a i)
                         (requires (wp (fun _ -> True) /\ (forall p1 p2. (forall x. p1 x ==> p2 x) ==> wp p1 ==> wp p2)))
                         (ensures (fun _ -> True))
@@ -97,51 +97,27 @@ let app #a #b #i (f : a -> GTD b i) (x : a) : GTD b i = f x
 
 // todo: use map/app from tot context and prove that it does what it's meant to do
 
-#set-options "--debug GT --debug_level SMTQuery"
-
-// GM: This fails, but I'm not sure why. With tactics (after compute) I see
-// the failing goal is
-//
-//  … @ …ido/r/fstar/layef/GT.fst(106,80-106,86)  Wed Jun 10 22:26:42 2020
-//  Goal 1/26
-//  a: Type
-//  i: idx
-//  n: nat
-//  f: _: a -> GT.GTD a i
-//  x: a
-//  x'0: nat
-//  uu___: l_True /\ l_True /\ ~(x'0 == 0)
-//  x'1: nat
-//  x'2: x'0 == x'1
-//  x'3: unit
-//  x'4: a
-//  --------------------------------------------------------------------------------
-//  squash (n - 1 >= 0)
-//  (*?u509*) _
-//
-// which seems odd, since [n] and [x'0] are disconnected.
-
 open FStar.Tactics
 
+[@@expect_failure]
 let rec appn #a #i (n:nat) (f : a -> GTD a i) (x : a) : GTD a i =
-  match n with 
+  match n with
   | 0 -> x
   | _ -> begin
     assume (n>0);
     appn (n-1) f (f x)
   end
 
-// explodes
-//[@@expect_failure]
-//let test #a #i (n:int) : GTD nat i =
-//  let r = app abs n in
-//  r
+[@@expect_failure]
+let test #a #i (n:int) : GTD nat i =
+  let r = app abs n in
+  r
 
 let labs0 #i (n:int) : GTD int i =
   if n < 0
   then -n
   else n
-  
+
 let labs #i (n:int) : GTD nat i =
   if n < 0
   then -n
@@ -149,6 +125,7 @@ let labs #i (n:int) : GTD nat i =
 
 // GM: This fails, which I think makes sense since the effect
 //     doesn't carry any logical payload, so the assume gets lost?
+[@@expect_failure]
 let test #a #i (n:int) : GTD nat i =
   let r = labs0 n in
   assume (r >= 0);
