examples/layeredeffects/ID1.fst
@@ -9,22 +9,31 @@ let monotonic (w:w0 'a) =
   forall p1 p2. (forall x. p1 x ==> p2 x) ==> w p1 ==> w p2
 
 val w (a : Type u#a) : Type u#(max 1 a)
-let w a = w:(w0 a){monotonic w}
+let w a = w:(w0 a) // {monotonic w}
 
 let repr (a : Type) (wp : w a) : Type =
   p:(pure_post a) -> squash (wp p) -> v:a{p v}
   //squash (exists p. wp p) -> v:a{forall p. wp p ==> p v}
 
-let return (a : Type) (x : a) : repr a (fun p -> p x) =
+let return_wp #a (x:a) : w a =
+  fun p -> p x
+
+let return (a : Type) (x : a) : repr a (return_wp x) =
  // Fun fact: using () instead of _ below makes us
  // lose the refinement and then this proof fails.
  // Keep that in mind all ye who enter here.
   fun p _ -> x
 
+let bind_wp #a #b
+  (wp_v : w a)
+  (wp_f : (x:a -> w b))
+  : w b
+  = fun p -> wp_v (fun x -> wp_f x p)
+
 let bind (a b : Type) (wp_v : w a) (wp_f: a -> w b)
     (v : repr a wp_v)
     (f : (x:a -> repr b (wp_f x)))
-: repr b (fun p -> wp_v (fun x -> wp_f x p))
+: repr b (bind_wp wp_v wp_f)
 = fun p _ -> f (v (fun x -> wp_f x p) ()) p () // explicit post is annoying
 
 let subcomp (a:Type) (wp1 wp2: w a)
@@ -34,8 +43,11 @@ let subcomp (a:Type) (wp1 wp2: w a)
        (ensures fun _ -> True)
 = f
 
+let ite_wp #a (wp1 wp2 : w a) (b : bool) : w a =
+  (fun p -> (b ==> wp1 p) /\ ((~b) ==> wp2 p))
+
 let if_then_else (a : Type) (wp1 wp2 : w a) (f : repr a wp1) (g : repr a wp2) (p : bool) : Type =
-  repr a (fun post -> (p ==> wp1 post) /\ ((~p) ==> wp2 post))
+  repr a (ite_wp wp1 wp2 p)
 
 // requires to prove that
 // p  ==> f <: (if_then_else p f g)
@@ -54,8 +66,8 @@ layered_effect {
        if_then_else = if_then_else
 }
 
-let lift_pure_nd (a:Type) (wp:pure_wp a{monotonic wp}) (f:(unit -> PURE a wp)) :
-  Pure (repr a wp) (requires True)
+let lift_pure_nd (a:Type) (wp:pure_wp a) (f:(eqtype_as_type unit -> PURE a wp)) :
+  Pure (repr a wp) (requires (monotonic wp))
                    (ensures (fun _ -> True))
   = fun p _ ->
     let r = f () in
@@ -76,7 +88,7 @@ effect Id (a:Type) (pre:pure_pre) (post:pure_post' a pre) =
 
 effect IdT (a:Type) = Id a True (fun _ -> True)
 
-(* Now works like a charm after fixing the lift from Pure *)
+[@@expect_failure] // why?
 let rec sum (l : list int) : IdT int
  =
   match l with
